work on lifting

concurrency/lifting.v
@@ -16,6 +16,48 @@ Require Import sepcomp.wholeprog_simulations. Import Wholeprog_sim.
 
 Require Import sepcomp.event_semantics.
 
+(** The X86 DryConc Machine*)
+Require Import concurrency.dry_context.
+
+Module lifting.  
+  Section lifting.
+
+
+    Notation GS := (eS.G).
+    Notation GT := (dry_context.SEM.G).    
+    Notation gT := (dry_context.the_ge).
+    
+    Notation semS := (eS.sem).
+    Notation semT := (dry_context.Sem dry.context SEM).
+
+    Notation CT := (dry_context.C).  
+
+    
+    Variable thread_sim : SM_simulation_inject (effsem semS) semT gS gT.
+
+    Definition ge_inv (geS : GS) (geT : GT) :=
+      genvs_domain_eq geS geT.
+
+    Definition init_inv j (geS : GS) valsS mS (geT : GT) valsT mT :=
+      Mem.mem_inj j mS mT /\
+      List.Forall2 (val_inject j) valsS valsT /\
+      Events.meminj_preserves_globals geS j.
+
+    Definition halt_inv j (geS : GS) rv1 mS (geT : GT) rv2 mT :=
+      Mem.mem_inj j mS mT /\
+      val_inject j rv1 rv2.
+    
+    Lemma concur_sim main p (sch : mySchedule.schedule) :
+      Wholeprog_sim
+        (source_concurrent_semantics sch p)
+        (target_concurrent_semantics sch p)
+        gS gT main
+        ge_inv init_inv halt_inv.
+    Proof. Admitted.
+  End lifting.
+End lifting.
+
+
 Record EvEffSem {G C} :=
   { (** [sem] is a memory semantics. *)
     esem : @EvSem G C;
